Test/civl/samples/treiber-stack.bpl
@@ -26,7 +26,7 @@ preserves call DomYieldInv#4();
   call loc_t := Alloc#0();
   ref_t := Ref(loc_t->val);
   call {:layer 4} Stack := Copy(Map_Update(Stack, ref_t, Vec_Empty()));
-  call {:layer 4} AbsLemma(ts->val[ref_t]->top, ts->val[ref_t]->stack->dom, ts->val[ref_t]->stack->val);
+  call {:layer 4} AbsLemma(ts->val->val[ref_t]->top, ts->val->val[ref_t]->stack->val);
 }
 
 atomic action {:layer 5} AtomicPush(ref_t: RefTreiber X, x: X) returns (success: bool)
@@ -43,17 +43,15 @@ preserves call YieldInv#4(ref_t);
 preserves call DomYieldInv#4();
 {
   var {:layer 4} old_top: RefNode X;
-  var {:layer 4} old_dom: [RefNode X]bool;
-  var {:layer 4} old_val: [RefNode X](Node X);
-  call {:layer 4} old_top := Copy(ts->val[ref_t]->top);
-  call {:layer 4} old_dom := Copy(ts->val[ref_t]->stack->dom);
-  call {:layer 4} old_val := Copy(ts->val[ref_t]->stack->val);
+  var {:layer 4} old_stack: Map (RefNode X) (Node X);
+  call {:layer 4} old_top := Copy(ts->val->val[ref_t]->top);
+  call {:layer 4} old_stack := Copy(ts->val->val[ref_t]->stack->val);
   call success := PushIntermediate(ref_t, x);
   if (success) {
-    call {:layer 4} FrameLemma(old_top, old_dom, old_val, ts->val[ref_t]->stack->dom, ts->val[ref_t]->stack->val);
+    call {:layer 4} FrameLemma(old_top, old_stack, ts->val->val[ref_t]->stack->val);
     call {:layer 4} Stack := Copy(Map_Update(Stack, ref_t, Vec_Append(Map_At(Stack, ref_t), x)));
-    assert {:layer 4} ts->val[ref_t]->top != Nil();
-    call {:layer 4} AbsLemma(ts->val[ref_t]->top, ts->val[ref_t]->stack->dom, ts->val[ref_t]->stack->val);
+    assert {:layer 4} ts->val->val[ref_t]->top != Nil();
+    call {:layer 4} AbsLemma(ts->val->val[ref_t]->top, ts->val->val[ref_t]->stack->val);
   }
 }
 
@@ -75,7 +73,7 @@ preserves call YieldInv#3(ref_t);
 preserves call YieldInv#4(ref_t);
 preserves call DomYieldInv#4();
 {
-  call {:layer 4} AbsLemma(ts->val[ref_t]->top, ts->val[ref_t]->stack->dom, ts->val[ref_t]->stack->val);
+  call {:layer 4} AbsLemma(ts->val->val[ref_t]->top, ts->val->val[ref_t]->stack->val);
   call success, x := PopIntermediate(ref_t);
   if (success) {
     assert {:layer 4} Vec_Len(Map_At(Stack, ref_t)) > 0;
@@ -87,12 +85,12 @@ atomic action {:layer 4} AtomicPopIntermediate(ref_t: RefTreiber X) returns (suc
 modifies ts;
 {
   var new_ref_n: RefNode X;
-  assume ts->dom[ref_t];
+  assume Map_Contains(ts->val, ref_t);
   if (success) {
-    assume ts->val[ref_t]->top != Nil();
-    assume ts->val[ref_t]->stack->dom[ts->val[ref_t]->top];
-    Node(new_ref_n, x) := ts->val[ref_t]->stack->val[ts->val[ref_t]->top];
-    ts->val[ref_t]->top := new_ref_n;
+    assume ts->val->val[ref_t]->top != Nil();
+    assume Map_Contains(ts->val->val[ref_t]->stack->val, ts->val->val[ref_t]->top);
+    Node(new_ref_n, x) := ts->val->val[ref_t]->stack->val->val[ts->val->val[ref_t]->top];
+    ts->val->val[ref_t]->top := new_ref_n;
   }
 }
 yield procedure {:layer 3} PopIntermediate(ref_t: RefTreiber X) returns (success: bool, x: X)
@@ -121,12 +119,12 @@ modifies ts;
   var t: RefNode X;
 
   if (success) {
-    t := ts->val[ref_t]->top;
+    t := ts->val->val[ref_t]->top;
     call new_loc_n, lmap_n := Lmap_Alloc(Node(t, x));
-    call Lmap_Assume(lmap_n, ts->val[ref_t]->stack);
-    ts->val[ref_t]->top := Ref(new_loc_n->val);
-    call lmap_n, lmap_n' := Lmap_Move(lmap_n, ts->val[ref_t]->stack, ts->val[ref_t]->top);
-    ts->val[ref_t]->stack := lmap_n';
+    call Lmap_Assume(lmap_n, ts->val->val[ref_t]->stack);
+    ts->val->val[ref_t]->top := Ref(new_loc_n->val);
+    call lmap_n, lmap_n' := Lmap_Move(lmap_n, ts->val->val[ref_t]->stack, ts->val->val[ref_t]->top);
+    ts->val->val[ref_t]->stack := lmap_n';
   }
 }
 yield procedure {:layer 2} PushIntermediate(ref_t: RefTreiber X, x: X) returns (success: bool)
@@ -140,7 +138,7 @@ preserves call YieldInv#2(ref_t);
 
   call ref_n := ReadTopOfStack#Push(ref_t);
   call new_loc_n, lmap_n := Lmap_Alloc(Node(ref_n, x));
-  call {:layer 2} Lmap_Assume(lmap_n, ts->val[ref_t]->stack);
+  call {:layer 2} Lmap_Assume(lmap_n, ts->val->val[ref_t]->stack);
   new_ref_n := Ref(new_loc_n->val);
   call success := WriteTopOfStack(ref_t, ref_n, new_ref_n);
   if (success) {
@@ -150,7 +148,7 @@ preserves call YieldInv#2(ref_t);
 
 right action {:layer 3} AtomicReadTopOfStack#Pop(ref_t: RefTreiber X) returns (ref_n: RefNode X)
 {
-  assert ts->dom[ref_t];
+  assert Map_Contains(ts->val, ref_t);
   assume NilDomain(ts, ref_t)[ref_n];
 }
 yield procedure {:layer 2} ReadTopOfStack#Pop(ref_t: RefTreiber X) returns (ref_n: RefNode X)
@@ -162,7 +160,7 @@ preserves call YieldInv#2(ref_t);
 
 right action {:layer 2} AtomicReadTopOfStack#Push(ref_t: RefTreiber X) returns (ref_n: RefNode X)
 {
-  assert ts->dom[ref_t];
+  assert Map_Contains(ts->val, ref_t);
 }
 yield procedure {:layer 1} ReadTopOfStack#Push(ref_t: RefTreiber X) returns (ref_n: RefNode X)
 refines AtomicReadTopOfStack#Push;
@@ -172,17 +170,17 @@ refines AtomicReadTopOfStack#Push;
 
 atomic action {:layer 1, 2} AtomicReadTopOfStack(ref_t: RefTreiber X) returns (ref_n: RefNode X)
 {
-  assert ts->dom[ref_t];
-  ref_n := ts->val[ref_t]->top;
+  assert Map_Contains(ts->val, ref_t);
+  ref_n := ts->val->val[ref_t]->top;
 }
 yield procedure {:layer 0} ReadTopOfStack(ref_t: RefTreiber X) returns (ref_n: RefNode X);
 refines AtomicReadTopOfStack;
 
 right action {:layer 3} AtomicLoadNode(ref_t: RefTreiber X, ref_n: RefNode X) returns (node: Node X)
 {
-  assert ts->dom[ref_t];
-  assert ts->val[ref_t]->stack->dom[ref_n];
-  node := ts->val[ref_t]->stack->val[ref_n];
+  assert Map_Contains(ts->val, ref_t);
+  assert Map_Contains(ts->val->val[ref_t]->stack->val, ref_n);
+  node := ts->val->val[ref_t]->stack->val->val[ref_n];
 }
 yield procedure {:layer 2} LoadNode(ref_t: RefTreiber X, ref_n: RefNode X) returns (node: Node X)
 refines AtomicLoadNode;
@@ -193,9 +191,9 @@ preserves call YieldInv#2(ref_t);
 
 atomic action {:layer 1,2} AtomicLoadNode#0(ref_t: RefTreiber X, ref_n: RefNode X) returns (node: Node X)
 {
-  assume ts->dom[ref_t];
-  assume ts->val[ref_t]->stack->dom[ref_n];
-  node := ts->val[ref_t]->stack->val[ref_n];
+  assume Map_Contains(ts->val, ref_t);
+  assume Map_Contains(ts->val->val[ref_t]->stack->val, ref_n);
+  node := ts->val->val[ref_t]->stack->val->val[ref_n];
 }
 yield procedure {:layer 0} LoadNode#0(ref_t: RefTreiber X, ref_n: RefNode X) returns (node: Node X);
 refines AtomicLoadNode#0;
@@ -204,9 +202,9 @@ left action {:layer 1, 2} AtomicAllocInStack(ref_t: RefTreiber X, ref_n: RefNode
 modifies ts;
 {
   var lmap_n', lmap_n'': Lheap (Node X);
-  assert ts->dom[ref_t];
-  call lmap_n'', lmap_n' := Lmap_Move(lmap_n, ts->val[ref_t]->stack, ref_n);
-  ts->val[ref_t]->stack := lmap_n';
+  assert Map_Contains(ts->val, ref_t);
+  call lmap_n'', lmap_n' := Lmap_Move(lmap_n, ts->val->val[ref_t]->stack, ref_n);
+  ts->val->val[ref_t]->stack := lmap_n';
 }
 yield procedure {:layer 0} AllocInStack(ref_t: RefTreiber X, ref_n: RefNode X, {:linear_in} lmap_n: Lheap (Node X));
 refines AtomicAllocInStack;
@@ -228,10 +226,10 @@ atomic action {:layer 1, 3} AtomicWriteTopOfStack(ref_t: RefTreiber X, old_ref_n
 modifies ts;
 {
   var top: RefNode X;
-  assert ts->dom[ref_t];
-  top := ts->val[ref_t]->top;
+  assert Map_Contains(ts->val, ref_t);
+  top := ts->val->val[ref_t]->top;
   if (old_ref_n == top) {
-    ts->val[ref_t]->top := new_ref_n;
+    ts->val->val[ref_t]->top := new_ref_n;
     r := true;
   }
   else {
@@ -259,70 +257,70 @@ yield procedure {:layer 0} Alloc#0() returns (loc_t: Lval (Loc (Treiber X)));
 refines AtomicAlloc#0;
 
 function {:inline} NilDomain(ts: Lheap (Treiber X), ref_t: RefTreiber X): [RefNode X]bool {
-  ts->val[ref_t]->stack->dom[Nil() := true]
+  ts->val->val[ref_t]->stack->val->dom->val[Nil() := true]
 }
 
 yield invariant {:layer 1} YieldInv#1(ref_t: RefTreiber X, ref_n: RefNode X);
-invariant ts->dom[ref_t];
-invariant ts->val[ref_t]->stack->dom[ref_n];
+invariant Map_Contains(ts->val, ref_t);
+invariant ts->val->val[ref_t]->stack->val->dom->val[ref_n];
 
 yield invariant {:layer 2} YieldInv#2(ref_t: RefTreiber X);
-invariant ts->dom[ref_t];
-invariant NilDomain(ts, ref_t)[ts->val[ref_t]->top];
+invariant Map_Contains(ts->val, ref_t);
+invariant NilDomain(ts, ref_t)[ts->val->val[ref_t]->top];
 
 yield invariant {:layer 3} YieldInv#3(ref_t: RefTreiber X);
-invariant ts->dom[ref_t];
-invariant NilDomain(ts, ref_t)[ts->val[ref_t]->top];
-invariant (forall ref_n: RefNode X :: ts->val[ref_t]->stack->dom[ref_n] ==> NilDomain(ts, ref_t)[ts->val[ref_t]->stack->val[ref_n]->next]);
+invariant Map_Contains(ts->val, ref_t);
+invariant NilDomain(ts, ref_t)[ts->val->val[ref_t]->top];
+invariant (var t := ts->val->val[ref_t]; (var m := t->stack->val; (forall ref_n: RefNode X :: m->dom->val[ref_n] ==> NilDomain(ts, ref_t)[m->val[ref_n]->next])));
 
 // The following is a manual encoding of the termination proof for the abstraction.
-function Abs(ref_n: RefNode X, dom: [RefNode X]bool, val:[RefNode X](Node X)): Vec X;
+function Abs(ref_n: RefNode X, map: Map (RefNode X) (Node X)): Vec X;
 
-pure procedure AbsCompute(ref_n: RefNode X, dom: [RefNode X]bool, val:[RefNode X](Node X)) returns (absStack: Vec X)
-requires Between(val, ref_n, ref_n, Nil());
-requires Subset(BetweenSet(val, ref_n, Nil()), dom[Nil() := true]);
+pure procedure AbsCompute(ref_n: RefNode X, map: Map (RefNode X) (Node X)) returns (absStack: Vec X)
+requires Between(map->val, ref_n, ref_n, Nil());
+requires Subset(BetweenSet(map->val, ref_n, Nil()), map->dom->val[Nil() := true]);
 ensures absStack ==
         if ref_n == Nil() then
         Vec_Empty() else
-        (var n := val[ref_n]; Vec_Append(Abs(n->next, dom, val), n->val));
-free ensures absStack == Abs(ref_n, dom, val);
+        (var n := Map_At(map, ref_n); Vec_Append(Abs(n->next, map), n->val));
+free ensures absStack == Abs(ref_n, map);
 {
   var n: Node X;
   if (ref_n == Nil()) {
       absStack := Vec_Empty();
   } else {
-      assert dom[ref_n]; // soundness of framing
-      n := val[ref_n];
-      assert Between(val, ref_n, n->next, Nil()); // soundness of termination (for induction)
-      call absStack := AbsCompute(n->next, dom, val);
+      assert Map_Contains(map, ref_n); // soundness of framing
+      n := Map_At(map, ref_n);
+      assert Between(map->val, ref_n, n->next, Nil()); // soundness of termination (for induction)
+      call absStack := AbsCompute(n->next, map);
       absStack := Vec_Append(absStack, n->val);
   }
 }
 
-pure procedure AbsLemma(ref_n: RefNode X, dom: [RefNode X]bool, val:[RefNode X](Node X))
-requires Between(val, ref_n, ref_n, Nil());
-requires Subset(BetweenSet(val, ref_n, Nil()), dom[Nil() := true]);
-ensures Abs(ref_n, dom, val) ==
+pure procedure AbsLemma(ref_n: RefNode X, map: Map (RefNode X) (Node X))
+requires Between(map->val, ref_n, ref_n, Nil());
+requires Subset(BetweenSet(map->val, ref_n, Nil()), map->dom->val[Nil() := true]);
+ensures Abs(ref_n, map) ==
         if ref_n == Nil() then
         Vec_Empty() else
-        (var n := val[ref_n]; Vec_Append(Abs(n->next, dom, val), n->val));
+        (var n := Map_At(map, ref_n); Vec_Append(Abs(n->next, map), n->val));
 {
   var absStack: Vec X;
-  call absStack := AbsCompute(ref_n, dom, val);
+  call absStack := AbsCompute(ref_n, map);
 }
 
-pure procedure FrameLemma(ref_n: RefNode X, dom: [RefNode X]bool, val: [RefNode X](Node X), dom': [RefNode X]bool, val': [RefNode X](Node X));
-requires Between(val, ref_n, ref_n, Nil());
-requires Subset(BetweenSet(val, ref_n, Nil()), dom[Nil() := true]);
-requires Subset(dom, dom');
-requires MapIte(dom, val, MapConst(Default())) == MapIte(dom, val', MapConst(Default()));
-ensures Abs(ref_n, dom, val) == Abs(ref_n, dom', val');
+pure procedure FrameLemma(ref_n: RefNode X, map: Map (RefNode X) (Node X), map': Map (RefNode X) (Node X));
+requires Between(map->val, ref_n, ref_n, Nil());
+requires Subset(BetweenSet(map->val, ref_n, Nil()), map->dom->val[Nil() := true]);
+requires Subset(map->dom->val, map'->dom->val);
+requires MapIte(map->dom->val, map->val, MapConst(Default())) == MapIte(map->dom->val, map'->val, MapConst(Default()));
+ensures Abs(ref_n, map) == Abs(ref_n, map');
 
 yield invariant {:layer 4} YieldInv#4(ref_t: RefTreiber X);
-invariant ts->dom[ref_t];
-invariant Map_At(Stack, ref_t) == (var t := ts->val[ref_t]; Abs(t->top, t->stack->dom, t->stack->val));
-invariant (var t := ts->val[ref_t]; Between(t->stack->val, t->top, t->top, Nil()));
-invariant (var t := ts->val[ref_t]; Subset(BetweenSet(t->stack->val, t->top, Nil()), NilDomain(ts, ref_t)));
+invariant Map_Contains(ts->val, ref_t);
+invariant Map_At(Stack, ref_t) == (var t := ts->val->val[ref_t]; Abs(t->top, t->stack->val));
+invariant (var t := ts->val->val[ref_t]; Between(t->stack->val->val, t->top, t->top, Nil()));
+invariant (var t := ts->val->val[ref_t]; Subset(BetweenSet(t->stack->val->val, t->top, Nil()), NilDomain(ts, ref_t)));
 
 yield invariant {:layer 4} DomYieldInv#4();
-invariant Stack->dom->val == ts->dom;
+invariant Stack->dom == ts->val->dom;
